why is the tactic script failing?

src/certigrad/aevb/grads_correct.lean
@@ -9,29 +9,34 @@ applied to the naive variational encoder.
 import .util .naive ..prove_model_ok ..pre ..backprop_correct
 
 set_option max_memory 4096
---set_option pp.max_depth 100000
---set_option pp.max_steps 10000000
 
 namespace certigrad
 namespace aevb
 
 open graph list tactic certigrad.tactic
 
-private meta def prove_indep_hyps (g fdict : expr) : tactic unit :=
-do to_expr ```((%%g)^.targets ⊆ env.keys %%fdict) >>= assert `H_tgts_ss_inputs,
+section proof
+parameters (a : arch) (ws : weights a) (x_data : T [a^.n_in, a^.n_x])
+def g := reparam (integrate_kl $ graph_naive a x_data)
+def fdict := mk_input_dict ws g
+
+attribute [cgsimp] g fdict
+
+private meta def prove_indep_hyps : tactic unit :=
+do to_expr ```((g a x_data)^.targets ⊆ env.keys (fdict a ws x_data)) >>= assert `H_tgts_ss_inputs,
      solve1 cgsimp,
-   to_expr ```(pdfs_exist_at (%%g)^.nodes %%fdict) >>= assert `H_pdfs_exist,
+   to_expr ```(pdfs_exist_at (g a x_data)^.nodes (fdict a ws x_data)) >>= assert `H_pdfs_exist,
      solve1 cgsimp
 
-private meta def prove_dep_hyps (g fdict tgt : expr) : tactic unit :=
-do to_expr ```(well_formed_at (%%g)^.costs (%%g)^.nodes %%fdict %%tgt) >>= assert `H_wf,
-     solve1 (dsimp >> constructor >> all_goals cgsimp),
-   to_expr ```(grads_exist_at (%%g)^.nodes %%fdict %%tgt) >>= assert `H_gs_exist,
-     solve1 (dsimp >> cgsimp),
-   to_expr ```(is_gintegrable (λ m, ⟦compute_grad_slow (%%g)^.costs (%%g)^.nodes m %%tgt⟧) %%fdict (%%g)^.nodes dvec.head) >>= assert `H_gint,
-     solve1 (dsimp >> cgsimp >> prove_is_mvn_integrable),
-   to_expr ```(can_differentiate_under_integrals (%%g)^.costs (%%g)^.nodes %%fdict %%tgt) >>= assert `H_can_diff,
-     solve1 (dsimp >> cgsimp >> prove_is_mvn_uintegrable)
+private meta def prove_dep_hyps (tgt : expr) : tactic unit :=
+do to_expr ```(well_formed_at (g a x_data)^.costs (g a x_data)^.nodes (fdict a ws x_data) %%tgt) >>= assert `H_wf,
+     solve1 (constructor >> all_goals cgsimp),
+   to_expr ```(grads_exist_at (g a x_data)^.nodes (fdict a ws x_data) %%tgt) >>= assert `H_gs_exist,
+     solve1 (cgsimp),
+   to_expr ```(is_gintegrable (λ m, ⟦compute_grad_slow (g a x_data)^.costs (g a x_data)^.nodes m %%tgt⟧) (fdict a ws x_data) (g a x_data)^.nodes dvec.head) >>= assert `H_gint,
+     solve1 (cgsimp >> prove_is_mvn_integrable),
+   to_expr ```(can_differentiate_under_integrals (g a x_data)^.costs (g a x_data)^.nodes (fdict a ws x_data) %%tgt) >>= assert `H_can_diff,
+     solve1 (cgsimp >> prove_is_mvn_uintegrable)
 
 private meta def forall_idxs (tac_base tac_step : tactic unit) : expr → tactic unit
 | idx :=
@@ -45,46 +50,32 @@ do exfalso,
    H_at_idx ← get_local `H_at_idx,
    to_expr ```(list.at_idx_over H_at_idx dec_trivial) >>= exact
 
-private meta def prove_aevb_step (g fdict : expr) : tactic unit :=
+private meta def prove_aevb_step : tactic unit :=
 do H_at_idx ← get_local `H_at_idx,
    H ← mk_app `and.right [H_at_idx],
    rewrite_core reducible tt tt occurrences.all ff H,
    H_type ← infer_type H,
    (tgt, new_tgt) ← match_eq H_type,
-   prove_dep_hyps g fdict new_tgt,
-   to_expr ```(backprop_correct %%fdict (%%g)^.targets H_tgts_ss_inputs H_at_idx H_wf H_gs_exist H_gint H_can_diff) >>= exact
+   prove_dep_hyps new_tgt,
+   to_expr ```(backprop_correct (fdict a ws x_data) (g a x_data)^.targets H_tgts_ss_inputs H_at_idx H_wf H_gs_exist H_gint H_can_diff) >>= exact
 
 meta def prove_aevb_ok : tactic unit :=
 do -- introduce hypotheses
-   [g, fdict, tgt, idx, H_at_idx] ← intron 5 | failed,
-   -- create recreate useful let-bindings
-   g ← to_expr ```(reparam (integrate_kl $ graph_naive a x_data)),
-   fdict ← to_expr ```(mk_input_dict ws %%g),
+   [tgt, idx, H_at_idx] ← intros | failed,
    -- prove independent hyps once and for all
-   prove_indep_hyps g fdict,
+   prove_indep_hyps,
    -- repeated case-analysis on idx
-   forall_idxs prove_aevb_base (prove_aevb_step g fdict) idx
+   forall_idxs prove_aevb_base prove_aevb_step idx
 
 lemma aevb_backprop_correct (a : arch) (ws : weights a) (x_data : T [a^.n_in, a^.n_x]) :
-let g : graph := reparam (integrate_kl $ graph_naive a x_data) in
-let fdict : env := mk_input_dict ws g in
 ∀ (tgt : reference) (idx : ℕ) (H_at_idx : at_idx g^.targets idx tgt),
 ∇ (λ θ₀, E (graph.to_dist (λ m, ⟦sum_costs m g^.costs⟧) (env.insert tgt θ₀ fdict) g^.nodes) dvec.head) (env.get tgt fdict)
 =
-E (graph.to_dist (λ m, backprop g^.costs g^.nodes m g^.targets) fdict g^.nodes) (λ dict, dvec.get tgt.2 dict idx)
-:=
+E (graph.to_dist (λ m, backprop g^.costs g^.nodes m g^.targets) fdict g^.nodes) (λ dict, dvec.get tgt.2 dict idx) :=
 begin
 prove_aevb_ok
 end
-/-
-| tgt 0     H_at_idx := begin prove_aevb_ok (dnth g^.targets 0) end
-| tgt 1     H_at_idx := begin prove_aevb_ok (dnth g^.targets 1) end
-| tgt 2     H_at_idx := begin prove_aevb_ok (dnth g^.targets 2) end
-| tgt 3     H_at_idx := begin prove_aevb_ok (dnth g^.targets 3) end
-| tgt 4     H_at_idx := begin prove_aevb_ok (dnth g^.targets 4) end
-| tgt (n+5) H_at_idx := false.rec _ (at_idx_over H_at_idx (by dec_triv))
--/
-#exit
 
+end proof
 end aevb
 end certigrad
